Added an example of the recursive variant of the mapper client

theories/logrel/examples/mapper.v
@@ -5,16 +5,23 @@ From iris.proofmode Require Import tactics.
 Section with_Σ.
   Context `{heapG Σ, chanG Σ}.
 
+  Definition mapper_client_type_aux (rec : lsty Σ) : lsty Σ :=
+    <!!> TY (lty_int ⊸ lty_bool); <!!> TY lty_int; <??> TY lty_bool; rec.
   Definition mapper_client_type : lsty Σ :=
-    <!!> TY (lty_int ⊸ lty_bool); <!!> TY lty_int; <??> TY lty_bool; END.
+    mapper_client_type_aux END.
 
-  Definition mapper_client : expr := λ: "c",
-    let: "f" := send "c" (λ: "x", #9000 < "x") in
-    let: "v" := send "c" #42 in
-    recv "c".
+  Instance mapper_client_type_contractive : Contractive mapper_client_type_aux.
+  Proof. solve_proto_contractive. Qed.
+
+  Definition mapper_client_rec_type : lsty Σ :=
+    lty_rec mapper_client_type_aux.
 
   Definition mapper_service_type : lsty Σ :=
     <??> TY (lty_int ⊸ lty_bool); <??> TY lty_int; <!!> TY lty_bool; END.
+
+  Definition mapper_client : expr := λ: "c",
+    send "c" (λ: "x", #9000 < "x");;
+    send "c" #42;; recv "c".
 
   Definition mapper_service : expr := λ: "c",
     let: "f" := recv "c" in
@@ -39,10 +46,8 @@ Section with_Σ.
     rewrite insert_insert /=.
     iApply ltyped_let.
     { iApply ltyped_send. apply lookup_insert.
-      rewrite insert_commute=> //.
       iApply ltyped_int. }
-    rewrite insert_insert /= (insert_commute _ "v" "c") //.
-    iApply ltyped_recv. apply lookup_insert.
+    rewrite insert_insert /=. iApply ltyped_recv. apply lookup_insert.
   Qed.
 
   Lemma mapper_service_typed Γ :
@@ -73,6 +78,73 @@ Section with_Σ.
         { iApply env_split_right=> //; last by iApply env_split_id_r. eauto. }
     }
     { iApply env_split_right=> //; last by iApply env_split_id_r. eauto. }
+  Qed.
+
+  Definition mapper_client_rec : expr := λ: "c",
+    send "c" (λ: "x", #9000 < "x");; send "c" #42;;
+    let: "x" := recv "c" in
+    send "c" (λ: "x", #4500 < "x");; send "c" #20;;
+    let: "y" := recv "c" in
+    ("x","y").
+
+  Lemma lty_le_rec_unfold_l {k} (C : lty Σ k → lty Σ k) `{!Contractive C} :
+    ⊢ lty_rec C <: C (lty_rec C).
+  Proof. iApply lty_le_l. iApply lty_le_rec_unfold. iApply lty_le_refl. Qed.
+
+  Lemma mapper_client_rec_typed Γ :
+    ⊢ Γ ⊨ mapper_client_rec :
+      (lty_chan (mapper_client_rec_type) ⊸ (lty_bool * lty_bool))%lty ⫤ Γ.
+  Proof.
+    iApply (ltyped_frame _ _ _ _ Γ).
+    { iApply env_split_id_l. }
+    2: { iApply env_split_id_l. }
+    iApply (ltyped_subsumption _ _ _((lty_chan (mapper_client_type_aux (mapper_client_type_aux (mapper_client_rec_type)))) ⊸ _)).
+    { iApply lty_le_arr.
+      - iNext. iApply lty_le_chan. iNext.
+        iApply lty_le_trans. iApply lty_le_rec_unfold_l.
+        do 3 iModIntro. iApply lty_le_rec_unfold_l.
+      - iApply lty_le_refl. }
+    iApply ltyped_lam.
+    iApply ltyped_let.
+    { iApply ltyped_send. apply lookup_insert.
+      iApply (ltyped_frame _ _ _ _ {["c":=_]}).
+      { iApply env_split_id_l. }
+      { iApply ltyped_lam. iApply ltyped_bin_op.
+        - iApply ltyped_var. apply lookup_insert.
+        - iApply ltyped_int. }
+      { iApply env_split_id_l. } }
+    rewrite insert_insert /=.
+    iApply ltyped_let.
+    { iApply ltyped_send. apply lookup_insert.
+      iApply ltyped_int. }
+    rewrite insert_insert /=.
+    iApply ltyped_let.
+    { iApply ltyped_recv. apply lookup_insert. }
+    rewrite insert_insert /=.
+    rewrite (insert_commute _ "x" "c") //.
+    iApply ltyped_let.
+    { iApply ltyped_send. apply lookup_insert.
+      iApply (ltyped_frame _ _ _ _ (<["c":=_]>(<["x":=_]>∅))).
+      { iApply env_split_id_l. }
+      { iApply ltyped_lam. iApply ltyped_bin_op.
+        - iApply ltyped_var. apply lookup_insert.
+        - iApply ltyped_int. }
+      { iApply env_split_id_l. } }
+    rewrite insert_insert /=.
+    iApply ltyped_let.
+    { iApply ltyped_send. apply lookup_insert.
+      iApply ltyped_int. }
+    rewrite insert_insert /=.
+    iApply ltyped_let.
+    { iApply ltyped_recv. apply lookup_insert. }
+    rewrite insert_insert /=.
+    iApply ltyped_pair.
+    - iApply ltyped_var. apply lookup_insert.
+    - rewrite (insert_commute _ "c" "x") //= (insert_commute _ "y" "x") //=.
+      iApply (ltyped_frame _ _ _ _ {["x":=_]}).
+      { iApply env_split_right=> //=. iApply env_split_id_r. }
+      iApply ltyped_var. apply lookup_insert.
+      iApply env_split_right=> //; last by iApply env_split_id_r=> //=. eauto.
   Qed.
 
 End with_Σ.
